<h2><a href="https://leetcode.com/problems/remove-palindromic-subsequences/">1332. Remove Palindromic Subsequences</a></h2><h3>Easy</h3><hr><div style="user-select: auto;"><p style="user-select: auto;">You are given a string <code style="user-select: auto;">s</code> consisting <strong style="user-select: auto;">only</strong> of letters <code style="user-select: auto;">'a'</code> and <code style="user-select: auto;">'b'</code>. In a single step you can remove one <strong style="user-select: auto;">palindromic subsequence</strong> from <code style="user-select: auto;">s</code>.</p>

<p style="user-select: auto;">Return <em style="user-select: auto;">the <strong style="user-select: auto;">minimum</strong> number of steps to make the given string empty</em>.</p>

<p style="user-select: auto;">A string is a <strong style="user-select: auto;">subsequence</strong> of a given string if it is generated by deleting some characters of a given string without changing its order. Note that a subsequence does <strong style="user-select: auto;">not</strong> necessarily need to be contiguous.</p>

<p style="user-select: auto;">A string is called <strong style="user-select: auto;">palindrome</strong> if is one that reads the same backward as well as forward.</p>

<p style="user-select: auto;">&nbsp;</p>
<p style="user-select: auto;"><strong style="user-select: auto;">Example 1:</strong></p>

<pre style="user-select: auto;"><strong style="user-select: auto;">Input:</strong> s = "ababa"
<strong style="user-select: auto;">Output:</strong> 1
<strong style="user-select: auto;">Explanation:</strong> s is already a palindrome, so its entirety can be removed in a single step.
</pre>

<p style="user-select: auto;"><strong style="user-select: auto;">Example 2:</strong></p>

<pre style="user-select: auto;"><strong style="user-select: auto;">Input:</strong> s = "abb"
<strong style="user-select: auto;">Output:</strong> 2
<strong style="user-select: auto;">Explanation:</strong> "<u style="user-select: auto;">a</u>bb" -&gt; "<u style="user-select: auto;">bb</u>" -&gt; "". 
Remove palindromic subsequence "a" then "bb".
</pre>

<p style="user-select: auto;"><strong style="user-select: auto;">Example 3:</strong></p>

<pre style="user-select: auto;"><strong style="user-select: auto;">Input:</strong> s = "baabb"
<strong style="user-select: auto;">Output:</strong> 2
<strong style="user-select: auto;">Explanation:</strong> "<u style="user-select: auto;">baa</u>b<u style="user-select: auto;">b</u>" -&gt; "<u style="user-select: auto;">b</u>" -&gt; "". 
Remove palindromic subsequence "baab" then "b".
</pre>

<p style="user-select: auto;">&nbsp;</p>
<p style="user-select: auto;"><strong style="user-select: auto;">Constraints:</strong></p>

<ul style="user-select: auto;">
	<li style="user-select: auto;"><code style="user-select: auto;">1 &lt;= s.length &lt;= 1000</code></li>
	<li style="user-select: auto;"><code style="user-select: auto;">s[i]</code> is either <code style="user-select: auto;">'a'</code> or <code style="user-select: auto;">'b'</code>.</li>
</ul>
</div>